theorem
  fixes a b::real
  assumes "b\<le>a"
    and "1<b"
  shows "ln (a/b) / ln a + ln (b/a) / ln b \<le>0" (is "?L \<le> _")
proof -
  (* Using logarithmic rules, we see that

  $\log_{a}a-\log_{a}b+\log_{b}b-\log_{b}a = 2-(\log_{a}b+\log_{b}a)$
  $=2-(\log_{a}b+\frac {1}{\log_{a}b})$ *)
  define x y where "x=ln a" and "y=ln b"
  have "y>0" using \<open>b>1\<close> unfolding y_def using ln_gt_zero sledgehammer
  moreover have "x\<ge>y" using \<open>a\<ge>b\<close> unfolding x_def y_def 
    using assms(2) sledgehammer
  ultimately have "x>0" sledgehammer
  have "?L = (x-y)/x + (y-x)/y"
    apply (subst (1 2) ln_div)
    using assms unfolding x_def y_def sledgehammer
  also have "... = 2 - (y/x + x/y)"
    sledgehammer
  also have "... \<le> 0"
  (* Since $a$ and $b$ are both greater than $1$, using [[AM-GM]] gives that the term in parentheses must be at least $2$, so the largest possible values is $2-2=0 \Rightarrow \textbf{B}.$ *)
  proof -
    have "0\<le> (sqrt (x/y) - sqrt (y/x))^2"
      sledgehammer
    also have "... = y/x + x/y -  2"
      unfolding power2_eq_square using \<open>x>0\<close> \<open>y>0\<close>
      sledgehammer
    finally show ?thesis sledgehammer
  qed
  finally show ?thesis .
qed